Finishes the proof of the constructive middle value theorem
git-svn-id: svn://scm.gforge.inria.fr/svnroot/cadcoq@91 c63750b6-0a05-0410-b89b-bf6a48017dd0

trunk/CAD_COQ/new_descartes/cmvt.v
@@ -1,4 +1,4 @@
-Require Import QArith List Omega ZArith pol.
+Require Import QArith List Omega ZArith pol Zwf Recdef.
 
 (* After a use of simpl, products of positive integers are replaced by
  products of positive numbers encapsulated in a Zpos constructor.  This
@@ -24,6 +24,13 @@ Ltac expand_Zpos_mult :=
   We first need a host of lemmas on the type of rational numbers, which
   is rather bare. *)
 
+Lemma Qmult_lt_0_compat :
+  forall x y, 0 < x -> 0 < y -> 0 < x * y.
+intros x y Hx Hy.
+assert (H0: 0 == 0 * y) by ring; rewrite H0.
+apply Qmult_lt_compat_r; auto.
+Qed.
+
 Definition Qmax (x y:Q) := if Qlt_le_dec x y then y else x.
 
 Lemma Qmax_le_l : forall x y, x <= Qmax x y.
@@ -34,6 +41,11 @@ Qed.
 Lemma Qmax_le_r : forall x y, y <= Qmax x y.
 intros x y; unfold Qmax; case (Qlt_le_dec x y); intro; apply Qle_refl || auto.
 Qed.
+
+Lemma neg_opp_pos : forall x, x < 0 -> 0 < - x.
+intros x; unfold Qlt, Qopp; simpl; intro; omega.
+Qed.
+
 
 Definition Qabs (x:Q) := Qmax x (-x).
 
@@ -76,13 +88,11 @@ replace ('(a2*d2))%Z with ('a2 *'d2)%Z by auto; ring.
 Qed.
 
 Lemma lt_opp_pos : forall x, -x < x -> 0 < x.
-intros x ltx; assert (H02 : 0 == 0*/(2#1)) by ring;
+intros x ltx; 
 assert (half_pos:0 < /(2#1)) by (unfold Qlt; simpl; omega).
-rewrite H02.
-assert (H1 : x == (x+x)*/(2#1))
-  by (unfold Qeq; simpl; expand_Zpos_mult; ring); rewrite H1; clear H1.
+setoid_replace x with ((x+x)*/(2#1)) by field.
+setoid_replace 0 with ((x+-x)*/(2#1)) by ring.
 apply Qmult_lt_compat_r; auto.
-assert (H0 : 0 == x + (-x)) by ring; rewrite H0; clear H0.
 apply Qplus_le_lt_compat; try apply Qle_refl; auto.
 Qed.
 
@@ -90,10 +100,9 @@ Lemma le_opp_pos : forall x, -x <= x -> 0 <= x.
 intros x lex; assert (H02 : 0 == 0*/(2#1)) by ring;
 assert (half_pos:0 <= /(2#1)) by (unfold Qle; simpl; omega).
 rewrite H02.
-assert (H1 : x == (x+x)*/(2#1))
-  by (unfold Qeq; simpl; expand_Zpos_mult; ring); rewrite H1; clear H1.
+setoid_replace x with ((x+x)*/(2#1)) by field.
 apply Qmult_le_compat_r; auto.
-assert (H0 : 0 == x + (-x)) by ring; rewrite H0; clear H0.
+setoid_replace 0 with (x+-x) by ring.
 apply Qplus_le_compat; try apply Qle_refl; auto.
 Qed.
 
@@ -106,9 +115,29 @@ Qed.
 
 Lemma Qopp_lt_compat : forall x y, x < y -> -y < -x.
 intros x y xy; rewrite <- (Qplus_0_r (-x));
- setoid_replace (-y) with (-x + (-y+x)) by ring.
+setoid_replace (-y) with (-x + (-y+x)) by ring.
 setoid_replace 0 with (-y + y) by ring.
 do 2 (apply Qplus_le_lt_compat; try apply Qle_refl); auto.
+Qed.
+
+Lemma Qopp_lt_lr : forall x y, x < - y -> y < - x.
+intros x y xy; setoid_replace y with (- - y) by ring.
+apply Qopp_lt_compat; assumption.
+Qed.
+
+Lemma Qopp_lt_rl : forall x y, -x < y -> - y < x.
+intros x y xy; setoid_replace x with (- - x) by ring.
+apply Qopp_lt_compat; assumption.
+Qed.
+
+Lemma Qopp_le_lr : forall x y, x <= - y -> y <= - x.
+intros x y xy; setoid_replace y with (- - y) by ring.
+apply Qopp_le_compat; assumption.
+Qed.
+
+Lemma Qopp_le_rl : forall x y, -x <= y -> - y <= x.
+intros x y xy; setoid_replace x with (- - x) by ring.
+apply Qopp_le_compat; assumption.
 Qed.
 
 Lemma pos_Qabs : forall x, 0 <= x -> Qabs x = x.
@@ -127,13 +156,6 @@ destruct x; unfold Qeq in Hx0; simpl in Hx0 |- *; rewrite Zmult_1_r in Hx0.
 rewrite Hx0; simpl; auto.
 Qed.
 
-(* Polynomial are only represented by the list of their coefficients.
-  To any polynomial, we associate the absolute polynomial, whose
-  coefficients are the absolute values of the initial coefficients. *)
-
-Fixpoint Qabs_pol (l:list Q) :list Q :=
- match l with nil => nil | a::tl => Qabs a::Qabs_pol tl end.
-
 Lemma opp_Qabs_le :  forall x, -x <= Qabs x.
 intros x; unfold Qabs, Qmax; case (Qlt_le_dec x (-x)); intro; auto;
  apply Qle_refl.
@@ -147,114 +169,41 @@ destruct (Qlt_le_dec (x * y) (-(x*y))) as [hp | hp]; try ring.
 assert (nx:0 < -x) by (apply lt_opp_pos; rewrite Qopp_opp; auto).
 assert (ny:0 < -y) by (apply lt_opp_pos; rewrite Qopp_opp; auto).
 case Qlt_not_le with (1:=hp).
-assert (q : -(x*y) == x * (-y)) by ring; rewrite q; clear q.
-assert (q : x*y == (-x * (-y))) by ring; rewrite q; clear q.
+setoid_replace (-(x*y)) with (x*(-y)) by ring.
+setoid_replace (x*y) with (-x*(-y)) by ring.
 apply Qmult_le_compat_r; apply Qlt_le_weak; auto.
 assert (nx:0 < -x) by (apply lt_opp_pos; rewrite Qopp_opp; auto).
 assert (py:0 <= y) by (apply le_opp_pos; auto).
 case (Qle_lt_or_eq _ _ py); intros hy'.
 case Qle_not_lt with (1:=hp).
-assert (q : -(x*y) == (-x) * y) by ring; rewrite q; clear q.
+setoid_replace (-(x*y)) with (-x*y) by ring.
 apply Qmult_lt_compat_r; auto.
 rewrite <- hy'; ring.
 assert (px:0<=x) by (apply le_opp_pos; auto).
 case (Qle_lt_or_eq _ _ px); intros hx'.
 case Qle_not_lt with (1:=hp).
-assert (q : -(x*y) == x * (-y)) by ring; rewrite q; clear q.
+setoid_replace (-(x*y)) with (x*(-y)) by ring.
 repeat rewrite (Qmult_comm x); apply Qmult_lt_compat_r; auto.
 rewrite <- hx'; ring.
 case (Qlt_not_le _ _ hp).
-assert (q : -(x*y) == (-x)*y) by ring; rewrite q; clear q.
+setoid_replace (-(x*y)) with (-x*y) by ring.
 apply Qmult_le_compat_r; auto; apply le_opp_pos; auto.
 Qed.
 
+Lemma Qabs_plus : forall x y, Qabs (x + y) <= Qabs x + Qabs y.
+intros x y; unfold Qabs, Qmax; case (Qlt_le_dec x (-x));
+ case (Qlt_le_dec y (-y)); case (Qlt_le_dec (x+y) (-(x+y))); 
+ try (setoid_replace (-(x+y)) with (-x+ -y) by ring);
+ try (intros; apply Qle_refl); intros xy xx yy.
 
-(* The value of the absolute polynomial is always larger than the value
- of the initial polynomial. *)
-
-Lemma Qabs_pol_bound :
-  forall l x, Qabs (eval_pol l x) <= eval_pol (Qabs_pol l) (Qabs x).
-induction l; intros x; simpl; unfold Qabs, Qmax.
-case (Qlt_le_dec 0 (-0)); simpl; intros; apply Qle_refl.
-destruct (Qlt_le_dec (a + x * eval_pol l x) (-(a+x*eval_pol l x))) as
- [test|test]; (case_eq (Qlt_le_dec a (-a)); [intros aneg ta | intros apos ta]);
-(case_eq (Qlt_le_dec x (-x)); [intros xneg tx | intros xpos tx]).
-rewrite Qopp_plus; apply Qplus_le_compat; try apply Qle_refl.
-assert (H0 : -(x*eval_pol l x)== -x *eval_pol l x) by ring;
-  rewrite H0;clear H0.
-repeat rewrite (Qmult_comm (-x));apply Qmult_le_compat_r.
-replace (-x) with (Qabs x) by (unfold Qabs, Qmax; rewrite tx; auto).
-apply Qle_trans with (Qabs (eval_pol l x)); auto.
-apply Qabs_le.
-replace (-x) with (Qabs x) by (unfold Qabs, Qmax; rewrite tx; auto).
-apply Qabs_le_0.
-rewrite Qopp_plus; apply Qplus_le_compat; try apply Qle_refl.
-assert (H0 : -(x*eval_pol l x)== x *-eval_pol l x) by ring;
-  rewrite H0;clear H0.
-repeat rewrite (Qmult_comm x);apply Qmult_le_compat_r.
-set (u:=-eval_pol l x);
-  replace x with (Qabs x) by (unfold Qabs, Qmax; rewrite tx; auto); unfold u.
-apply Qle_trans with (Qabs (eval_pol l x)); auto.
-apply opp_Qabs_le.
-replace x with (Qabs x) by (unfold Qabs, Qmax; rewrite tx; auto).
-apply Qabs_le_0.
-rewrite Qopp_plus; apply Qplus_le_compat; auto.
-assert (H0 : -(x*eval_pol l x)== -x *eval_pol l x) by ring;
-  rewrite H0;clear H0.
-repeat rewrite (Qmult_comm (-x));apply Qmult_le_compat_r.
-replace (-x) with (Qabs x) by (unfold Qabs, Qmax; rewrite tx; auto).
-apply Qle_trans with (Qabs (eval_pol l x)); auto.
-apply Qabs_le.
-replace (-x) with (Qabs x) by (unfold Qabs, Qmax; rewrite tx; auto).
-apply Qabs_le_0.
-rewrite Qopp_plus; apply Qplus_le_compat; auto.
-assert (H0 : -(x*eval_pol l x)== x *-eval_pol l x) by ring;
-  rewrite H0;clear H0.
-repeat rewrite (Qmult_comm x);apply Qmult_le_compat_r.
-set (u:=-eval_pol l x);
-  replace x with (Qabs x) by (unfold Qabs, Qmax; rewrite tx; auto); unfold u.
-apply Qle_trans with (Qabs (eval_pol l x)); auto.
-apply opp_Qabs_le.
-replace x with (Qabs x) by (unfold Qabs, Qmax; rewrite tx; auto);
-  apply Qabs_le_0.
-apply Qplus_le_compat; try (apply Qlt_le_weak; assumption).
-assert (H0 : x*eval_pol l x== -x *-eval_pol l x) by ring;
-  rewrite H0;clear H0.
-repeat rewrite (Qmult_comm (-x));apply Qmult_le_compat_r.
-replace (-x) with (Qabs x) by (unfold Qabs, Qmax; rewrite tx; auto).
-apply Qle_trans with (Qabs (eval_pol l x)); auto.
-apply opp_Qabs_le.
-replace (-x) with (Qabs x) by (unfold Qabs, Qmax; rewrite tx; auto).
-apply Qabs_le_0.
-apply Qplus_le_compat; try (apply Qlt_le_weak; assumption).
-repeat rewrite (Qmult_comm x);apply Qmult_le_compat_r.
-set (u:=eval_pol l x);
-  replace x with (Qabs x) by (unfold Qabs, Qmax; rewrite tx; auto); unfold u.
-apply Qle_trans with (Qabs (eval_pol l x)); auto.
-apply Qabs_le.
-replace x with (Qabs x) by (unfold Qabs, Qmax; rewrite tx; auto);
-  apply Qabs_le_0.
-apply Qplus_le_compat; try apply Qle_refl.
-assert (H0 : x*eval_pol l x== -x *-eval_pol l x) by ring;
-  rewrite H0;clear H0.
-repeat rewrite (Qmult_comm (-x));apply Qmult_le_compat_r.
-replace (-x) with (Qabs x) by (unfold Qabs, Qmax; rewrite tx; auto).
-apply Qle_trans with (Qabs (eval_pol l x)); auto.
-apply opp_Qabs_le.
-replace (-x) with (Qabs x) by (unfold Qabs, Qmax; rewrite tx; auto).
-apply Qabs_le_0.
-apply Qplus_le_compat; try apply Qle_refl.
-repeat rewrite (Qmult_comm x);apply Qmult_le_compat_r.
-set (u:=eval_pol l x);
-  replace x with (Qabs x) by (unfold Qabs, Qmax; rewrite tx; auto); unfold u.
-apply Qle_trans with (Qabs (eval_pol l x)); auto.
-apply Qabs_le.
-replace x with (Qabs x) by (unfold Qabs, Qmax; rewrite tx; auto);
-  apply Qabs_le_0.
-Qed.
-
-Lemma neg_opp_pos : forall x, x < 0 -> 0 < - x.
-intros x; unfold Qlt, Qopp; simpl; intro; omega.
+case (Qle_not_lt _ _ xy); apply Qplus_le_lt_compat; auto;
+ apply Qlt_le_weak; auto.
+repeat rewrite (Qplus_comm x); apply Qplus_le_compat; auto; apply Qle_refl.
+repeat rewrite <- (Qplus_comm y); apply Qplus_le_compat; 
+ try (apply Qlt_le_weak; solve[auto]); apply Qle_refl.
+apply Qplus_le_compat; auto; apply Qle_refl.
+apply Qplus_le_compat; try apply Qle_refl; apply Qlt_le_weak; auto.
+apply Qplus_le_compat; auto.
 Qed.
 
 Lemma Qabs_interval : forall x y z, x < y -> y < z ->
@@ -282,56 +231,101 @@ apply Qlt_le_trans with (Qabs z); try apply Qmax_le_r.
 rewrite pos_Qabs; auto; apply Qlt_le_weak; auto.
 Qed.
 
-(* A polynomial that has a negative value necessarily is not the null
- polynomial. *)
-
-Lemma cm1 :
-  forall l x y, eval_pol l x < eval_pol l y  -> exists a, l = a::(tail l).
-intros l; case l.
-simpl;intros x y abs; case (Qlt_not_le _ _ abs); apply Qle_refl.
-intros a l' x y _; exists a; auto.
+Lemma inv_pos : forall x, 0 < x -> 0 < /x.
+intros [ [| x| x] y]; unfold Qlt, Qinv; simpl; compute; auto.
 Qed.
 
-Lemma add_exists :
-  forall l1 l2, exists l', forall x, eval_pol l1 x + eval_pol l2 x ==
-  eval_pol l' x.
-induction l1 as [ | a l1 IHl1]; destruct l2 as [ | b l2].
-exists (@nil Q); simpl; intros; ring.
-exists (b::l2); simpl; intros; ring.
-exists (a::l1); simpl; intros; ring.
-destruct (IHl1 l2) as [l' q].
-exists ((a+b)::l'); simpl; intros; rewrite <- q; ring.
+Lemma Qabs_non_pos : forall x, Qabs x <= 0 -> x == 0.
+intros x; unfold Qabs, Qmax; case (Qlt_le_dec x (-x)).
+intros l1 l2; apply Qle_antisym; rewrite <- (Qopp_opp x); 
+rewrite <- (Qopp_opp 0); apply Qopp_le_compat; auto.
+apply le_opp_pos.
+rewrite Qopp_opp; apply Qlt_le_weak; auto.
+intros l1 l2; apply Qle_antisym; auto; apply le_opp_pos; auto.
 Qed.
 
-Lemma s_mult_exists :
-  forall a l, exists l', forall x, a * eval_pol l x == eval_pol l' x.
-intros a; induction l as [ | b l IHl]; simpl.
-exists (@nil Q); simpl; intros; ring.
-destruct IHl as [l' q]; exists ((a*b)::l'); simpl; intros; rewrite <- q; ring.
+Lemma Qmult_le_reg_r : forall a b, 0 < b -> 0 <= a * b -> 0 <= a.
+intros a b pb ab; assert (~ b==0) 
+  by (intros q; rewrite q in pb; discriminate pb).
+rewrite <- (Qdiv_mult_l a b); auto.
+assert (d0 : 0 == 0 * /b) by ring; rewrite d0; clear d0.
+unfold Qdiv; apply Qmult_le_compat_r; auto; 
+ apply Qlt_le_weak; apply inv_pos; auto.
 Qed.
 
-Lemma mult_exists :
-  forall l1 l2, exists l', forall x, eval_pol l1 x * eval_pol l2 x ==
-   eval_pol l' x.
-induction l1 as [ | a l1 IHl1].
-exists (@nil Q); simpl; intros; ring.
-simpl.
-intros l2; destruct (s_mult_exists a l2) as [l2a q].
-destruct (IHl1 (0::l2)) as [l1l2x q1].
-destruct (add_exists l1l2x l2a) as [l' q2].
-exists l'; simpl; intros.
-rewrite <- q2; rewrite <- q1; rewrite <- q; simpl; ring.
+Lemma Qmult_le_reg_l : forall a b, 0 < b -> 0 <= b * a -> 0 <= a.
+intros a b pb ab; apply (Qmult_le_reg_r a b); auto; rewrite Qmult_comm; auto.
 Qed.
 
-Lemma compose_exists :
-  forall l a, exists l', forall x, eval_pol l x == eval_pol l' (x - a).
-induction l as [ | b l IHl]; intros a; simpl.
-exists (@nil Q); simpl; intros; ring.
-destruct (IHl a) as [l' q].
-destruct (mult_exists (a::1::nil) l') as [l2 q2].
-destruct (add_exists (b::nil) l2) as [l3 q3].
-exists l3; intros x; rewrite <- q3; simpl;
-   rewrite <- q2; rewrite q; simpl; ring.
+(* Polynomial are only represented by the list of their coefficients.
+  To any polynomial, we associate the absolute polynomial, whose
+  coefficients are the absolute values of the initial coefficients. *)
+
+Fixpoint Qabs_pol (l:list Q) :list Q :=
+ match l with nil => nil | a::tl => Qabs a::Qabs_pol tl end.
+
+(* The value of the absolute polynomial is always larger than the value
+ of the initial polynomial. *)
+
+Hint Resolve Qabs_le Qabs_le_0 opp_Qabs_le Qle_refl Qlt_le_weak Qinv_lt_0_compat.
+
+Lemma Qabs_pol_bound :
+  forall l x, Qabs (eval_pol l x) <= eval_pol (Qabs_pol l) (Qabs x).
+induction l; intros x; simpl; unfold Qabs, Qmax;
+  try solve [case (Qlt_le_dec 0 (-0)); simpl; intros; apply Qle_refl].
+destruct (Qlt_le_dec (a + x * eval_pol l x) (-(a+x*eval_pol l x))) as
+ [test|test]; (case_eq (Qlt_le_dec a (-a)); [intros aneg ta | intros apos ta]);
+(case_eq (Qlt_le_dec x (-x)); [intros xneg tx | intros xpos tx]).
+rewrite Qopp_plus; apply Qplus_le_compat; try apply Qle_refl.
+setoid_replace (-(x*eval_pol l x)) with (-x*eval_pol l x) by ring.
+repeat rewrite (Qmult_comm (-x));apply Qmult_le_compat_r.
+replace (-x) with (Qabs x) by (unfold Qabs, Qmax; rewrite tx; auto).
+apply Qle_trans with (Qabs (eval_pol l x)); auto.
+replace (-x) with (Qabs x) by (unfold Qabs, Qmax; rewrite tx; auto); auto.
+rewrite Qopp_plus; apply Qplus_le_compat; try apply Qle_refl.
+setoid_replace (-(x*eval_pol l x)) with (x*-eval_pol l x) by ring.
+repeat rewrite (Qmult_comm x);apply Qmult_le_compat_r.
+set (u:=-eval_pol l x);
+  replace x with (Qabs x) by (unfold Qabs, Qmax; rewrite tx; auto); unfold u.
+apply Qle_trans with (Qabs (eval_pol l x)); auto.
+replace x with (Qabs x) by (unfold Qabs, Qmax; rewrite tx; auto); auto.
+rewrite Qopp_plus; apply Qplus_le_compat; auto.
+setoid_replace (-(x*eval_pol l x)) with (-x*eval_pol l x) by ring.
+repeat rewrite (Qmult_comm (-x));apply Qmult_le_compat_r.
+replace (-x) with (Qabs x) by (unfold Qabs, Qmax; rewrite tx; auto).
+apply Qle_trans with (Qabs (eval_pol l x)); auto.
+replace (-x) with (Qabs x) by (unfold Qabs, Qmax; rewrite tx; auto); auto.
+rewrite Qopp_plus; apply Qplus_le_compat; auto.
+setoid_replace (-(x*eval_pol l x)) with (x*-eval_pol l x) by ring.
+repeat rewrite (Qmult_comm x);apply Qmult_le_compat_r.
+set (u:=-eval_pol l x);
+  replace x with (Qabs x) by (unfold Qabs, Qmax; rewrite tx; auto); unfold u.
+apply Qle_trans with (Qabs (eval_pol l x)); auto.
+replace x with (Qabs x) by (unfold Qabs, Qmax; rewrite tx; auto); auto.
+apply Qplus_le_compat; try (apply Qlt_le_weak; assumption).
+setoid_replace (x*eval_pol l x) with (-x*-eval_pol l x) by ring.
+repeat rewrite (Qmult_comm (-x));apply Qmult_le_compat_r.
+replace (-x) with (Qabs x) by (unfold Qabs, Qmax; rewrite tx; auto).
+apply Qle_trans with (Qabs (eval_pol l x)); auto.
+replace (-x) with (Qabs x) by (unfold Qabs, Qmax; rewrite tx; auto); auto.
+apply Qplus_le_compat; try (apply Qlt_le_weak; assumption).
+repeat rewrite (Qmult_comm x);apply Qmult_le_compat_r.
+set (u:=eval_pol l x);
+  replace x with (Qabs x) by (unfold Qabs, Qmax; rewrite tx; auto); unfold u.
+apply Qle_trans with (Qabs (eval_pol l x)); auto.
+replace x with (Qabs x) by (unfold Qabs, Qmax; rewrite tx; auto);auto.
+apply Qplus_le_compat; try apply Qle_refl.
+setoid_replace (x*eval_pol l x) with (-x*-eval_pol l x) by ring.
+repeat rewrite (Qmult_comm (-x));apply Qmult_le_compat_r.
+replace (-x) with (Qabs x) by (unfold Qabs, Qmax; rewrite tx; auto).
+apply Qle_trans with (Qabs (eval_pol l x)); auto.
+replace (-x) with (Qabs x) by (unfold Qabs, Qmax; rewrite tx; auto); auto.
+apply Qplus_le_compat; try apply Qle_refl.
+repeat rewrite (Qmult_comm x);apply Qmult_le_compat_r.
+set (u:=eval_pol l x);
+  replace x with (Qabs x) by (unfold Qabs, Qmax; rewrite tx; auto); unfold u.
+apply Qle_trans with (Qabs (eval_pol l x)); auto.
+replace x with (Qabs x) by (unfold Qabs, Qmax; rewrite tx; auto); auto.
 Qed.
 
 Lemma Qabs_pol_pos :
@@ -355,6 +349,63 @@ apply Qmult_le_compat_r; auto.
 apply Qabs_pol_pos; apply Qle_trans with x; auto.
 Qed.
 
+(* A polynomial that has distinct values cannot be the null
+ polynomial. *)
+
+Lemma cm1 :
+  forall l x y, eval_pol l x < eval_pol l y  -> exists a, l = a::(tail l).
+intros l; case l.
+simpl;intros x y abs; case (Qlt_not_le _ _ abs); apply Qle_refl.
+intros a l' x y _; exists a; auto.
+Qed.
+
+(* To describe polynomial addition, multiplication by a scalar, and
+  multiplication, we simply specify these operations so that their
+  interpretation through polynomial evaluation returns the corresponding
+  scalar operation. *)
+
+Definition add_pol :
+  forall l1 l2, {l' | forall x, eval_pol l1 x + eval_pol l2 x ==
+  eval_pol l' x}.
+induction l1 as [ | a l1 IHl1]; destruct l2 as [ | b l2].
+exists (@nil Q); simpl; intros; ring.
+exists (b::l2); simpl; intros; ring.
+exists (a::l1); simpl; intros; ring.
+destruct (IHl1 l2) as [l' q].
+exists ((a+b)::l'); simpl; intros; rewrite <- q; ring.
+Defined.
+
+Definition s_mult_pol :
+  forall a l, {l' | forall x, a * eval_pol l x == eval_pol l' x}.
+intros a; induction l as [ | b l IHl]; simpl.
+exists (@nil Q); simpl; intros; ring.
+destruct IHl as [l' q]; exists ((a*b)::l'); simpl; intros; rewrite <- q; ring.
+Defined.
+
+Lemma mult_pol :
+  forall l1 l2, {l' | forall x, eval_pol l1 x * eval_pol l2 x ==
+   eval_pol l' x}.
+induction l1 as [ | a l1 IHl1].
+exists (@nil Q); simpl; intros; ring.
+simpl.
+intros l2; destruct (s_mult_pol a l2) as [l2a q].
+destruct (IHl1 (0::l2)) as [l1l2x q1].
+destruct (add_pol l1l2x l2a) as [l' q2].
+exists l'; simpl; intros.
+rewrite <- q2; rewrite <- q1; rewrite <- q; simpl; ring.
+Qed.
+
+Lemma translate_pol :
+  forall l a, exists l', forall x, eval_pol l x == eval_pol l' (x - a).
+induction l as [ | b l IHl]; intros a; simpl.
+exists (@nil Q); simpl; intros; ring.
+destruct (IHl a) as [l' q].
+destruct (mult_pol (a::1::nil) l') as [l2 q2].
+destruct (add_pol (b::nil) l2) as [l3 q3].
+exists l3; intros x; rewrite <- q3; simpl;
+   rewrite <- q2; rewrite q; simpl; ring.
+Qed.
+
 Add Morphism Qabs with signature Qeq ==> Qeq as Qabs_mor.
 intros x1 x2 x1x2; unfold Qabs, Qmax; 
   destruct (Qlt_le_dec x1 (-x1)) as [hx1 | hx1];
@@ -364,9 +415,15 @@ case Qlt_not_le with (1:= hx1); auto.
 case Qlt_not_le with (1:= hx2); auto.
 Qed.
 
+Add Morphism eval_pol with signature @eq (list Q) ==> Qeq ==> Qeq as eval_pol_mor.
+intros l x y; induction l.
+simpl; intros; apply Qeq_refl.
+simpl; intros Hxy; rewrite IHl; auto; rewrite Hxy; apply Qeq_refl.
+Qed.
+
 Lemma cm2 :
-  forall l b, exists c,
-  forall x, 0 <= x -> x <= b -> Qabs (eval_pol l x - eval_pol l 0) <= c * x.
+  forall l b, { c |
+  forall x, 0 <= x -> x <= b -> Qabs (eval_pol l x - eval_pol l 0) <= c * x}.
 intros l b.
 destruct l as [ | a l].
 exists 0; simpl; intros; ring_simplify; apply Qle_refl.
@@ -379,9 +436,9 @@ apply Qmult_le_compat_r; auto.
 apply Qle_trans with (2 := Qabs_pol_increase l x b px xb).
 pattern x at 2; replace x with (Qabs x); [apply Qabs_pol_bound | idtac].
 apply pos_Qabs; auto.
-Qed.
+Defined.
 
-Lemma QZ_bound : forall x:Q, 0 <= x -> exists n, x <= n#1.
+Lemma QZ_bound : forall x:Q, 0 <= x -> {n | x <= n#1}.
 intros [n d]; exists(Zdiv n (Zpos d)+1)%Z.
 assert (dpos : (('d) > 0)%Z) by apply (refl_equal Gt).
 unfold Qle; simpl; rewrite Zmult_1_r; rewrite Zmult_plus_distr_l.
@@ -389,7 +446,7 @@ pattern n at 1; rewrite (Z_div_mod_eq n ('d)); auto.
 rewrite (Zmult_comm ('d)); apply Zplus_le_compat; auto with zarith.
 rewrite Zmult_1_l; destruct (Z_mod_lt n ('d)) as [_ H2]; auto; 
 apply Zlt_le_weak; apply H2.
-Qed.
+Defined.
 
 Lemma Qdiv_lt_0_compat : forall x y, 0 < x -> 0 < y -> 0 < x / y.
 intros x [[ | p | p] d] Hx Hy; unfold Qdiv, Qinv; simpl.
@@ -400,40 +457,325 @@ apply Qmult_lt_compat_r; auto.
 unfold Qlt in Hy; simpl in Hy; discriminate Hy.
 Qed.
 
-(* 
-Lemma constructive_mvt :
-  forall l x y, x < y -> eval_pol l x < 0 -> 0 < eval_pol l y  ->
-       forall epsilon, 0 < epsilon ->
-       exists x', exists y',  -epsilon < eval_pol l x' /\
-         eval_pol l x' < 0 /\ 0 < eval_pol l y' /\
-         eval_pol l y' < epsilon /\ x < x' /\ x' < y' /\ y' < y.
-intros l a b ab nla plb.
-destruct (compose_exists l a) as [l' q].
-destruct (cm2 l' (b-a)) as [c pc].
-intros epsilon pe; destruct (QZ_bound ((b-a)*c/epsilon)) as [n qn].
-assert (alb : 0 < b -a ).
-assert (d0 : 0 == a - a) by ring; rewrite d0; unfold Qminus.
-repeat rewrite <- (Qplus_comm (-a)); apply Qplus_le_lt_compat; auto.
-apply Qle_refl.
-assert (ba:~ b-a == 0).
-intros abs; case (Qlt_not_eq 0 (b-a) alb).
-rewrite abs; apply Qeq_refl.
-assert (pc' : 0 <= c).
-assert (c': c == c * (b-a) * (1/(b-a))).
-rewrite <- Qmult_assoc; rewrite Qmult_div_r; auto.
-ring.
-rewrite c'; clear c'.
-assert (d0 : 0 == 0 *(1/(b-a))) by ring; rewrite d0; clear d0.
-apply Qmult_le_compat_r.
-assert (pc' := pc (b-a) (Qlt_le_weak _ _ alb) (Qle_refl _)).
-apply Qle_trans with (2:= pc'); apply Qabs_le_0.
-apply Qlt_le_weak; apply Qdiv_lt_0_compat; auto.
-unfold Qlt; simpl; omega.
-destruct (Qle_lt_or_eq _ _ pc') as [pc1 | pc1]; clear pc'; rename pc1 into pc'.
-apply Qlt_le_weak; apply Qdiv_lt_0_compat; auto.
-assert (q':0==0*c) by ring; rewrite q'; apply Qmult_lt_compat_r; auto.
-rewrite <- pc'; unfold Qdiv; ring_simplify; apply Qle_refl.
-assert (exists p:Z, eval_pol l (a + (p#1) * (epsilon/c)) < 0 /\
-         (exists b', 0 < eval_pol l b' /\ b' <= a + ((p+1)#1)*(epsilon/c))).
+Lemma cm3 :
+  forall b, 0 < b -> forall l, 
+   {c |
+    forall x y, 0 <= x -> x <= y -> y <= b -> 
+    Qabs (eval_pol l y - eval_pol l x) <= c*(y-x)}.
+intros b pb; induction l.
+exists 0; intros x y px xy yb; simpl; ring_simplify.
+assert (d0 : 0-0 == 0) by ring.
+rewrite d0; apply Qle_refl.
+destruct IHl as [c cp].
+exists (eval_pol (Qabs_pol l) b+c*b); intros x y px xy yb; simpl.
+match goal with |- Qabs (?e) <= _ =>
+  setoid_replace e with 
+     ((y-x)*eval_pol l y + x*(eval_pol l y - eval_pol l x)) by ring end.
+apply Qle_trans with
+   (1:= Qabs_plus ((y-x)*eval_pol l y) (x*(eval_pol l y - eval_pol l x))).
+rewrite Qmult_plus_distr_l; apply Qplus_le_compat.
+assert (xmy: 0 <= y - x).
+setoid_replace 0 with (x+ -x) by ring.
+unfold Qminus; apply Qplus_le_compat; auto.
+rewrite Qabs_mult; rewrite (pos_Qabs (y-x)); auto.
+rewrite (Qmult_comm (y-x)); apply Qmult_le_compat_r; auto.
+assert (py: 0 <= y) by (apply Qle_trans with x; auto).
+apply Qle_trans with (2:= Qabs_pol_increase l y b py yb).
+pattern y at 2; rewrite <- (pos_Qabs y py).
+apply Qabs_pol_bound.
+setoid_replace (c*b*(y-x)) with (b * (c*(y-x))) by ring.
+rewrite Qabs_mult; rewrite (pos_Qabs x px).
+apply Qle_trans with (b*Qabs (eval_pol l y - eval_pol l x)).
+apply Qmult_le_compat_r; auto.
+apply Qle_trans with y; auto.
+repeat rewrite (Qmult_comm b); apply Qmult_le_compat_r; auto.
+Qed.
 
-*)
+Definition find_pair : forall A:Type, forall P:A->Prop, forall Q:A->A->Prop,
+    forall l:list A, forall a b:A, P a -> ~P b ->
+    (forall l1 l2 x y, a::l++b::nil=l1++x::y::l2 -> Q x y) ->
+    (forall x, In x l -> {P x}+{~P x}) ->
+    {c :A & { d | Q c d /\ P c /\ ~P d}}.
+intros A P Q; induction l; simpl; intros a' b' Pa Pb connect dec.
+exists a'; exists b'; split; auto.
+apply (connect nil nil); auto.
+case (dec a); auto.
+intros Pa1; destruct (IHl a b' Pa1 Pb) as [c [d [cd [Pc Pd]]]].
+intros l1 l2 x y q; apply (connect (a'::l1) l2); rewrite q; simpl;auto.
+intros x inx; apply (dec x); auto.
+exists c; exists d; auto.
+exists a'; exists a; split; auto.
+apply (connect nil (l++b'::nil)); auto.
+Qed.
+
+Function ns (p n:Z) {measure Zabs_nat n} : list Z :=
+   if Z_le_dec n 0 then p::nil else (p-n)%Z::ns p (n-1)%Z.
+intros; apply Zabs_nat_lt; omega.
+Defined.
+
+Lemma ns_head : forall p n, (0 <= n)%Z -> exists l, ns p n = (p - n)%Z::l.
+intros p n; functional induction ns p n.
+intros; assert (n = 0)%Z by omega; subst n; ring_simplify (p-0)%Z; exists nil; auto.
+intros _; destruct IHl  as [l' pl'].
+omega.
+exists ((p-(n-1))%Z::l'); rewrite pl'; auto.
+Qed.
+
+Lemma ns_step : forall p n, forall l1 l2 x y, (0 <= n)%Z ->
+  ns p n = l1++x::y::l2 -> y = (x + 1)%Z.
+intros p n; functional induction ns p n.
+intros; repeat (destruct l1; try discriminate).
+assert (np1 : (0 <= n-1)%Z) by omega.
+intros l1 l2 x y np q; destruct l1 as [ | a l1].
+destruct (ns_head p (n-1)  np1) as [l' ql'].
+rewrite ql' in q; simpl in q; injection q; intros; subst y x; ring.
+apply (IHl l1 l2); auto.
+simpl in q; injection q; auto.
+Qed.
+
+Lemma ns_tail : forall p n, exists l, ns p n = l++p::nil.
+intros p n; functional induction ns p n.
+exists nil; auto.
+destruct IHl as [l ql]; rewrite ql; exists ((p-n)%Z::l); auto.
+Qed.
+
+Lemma ns_bounds : forall p n x l1 l2, (0 <= n)%Z -> ns p n = l1++x::l2 -> 
+        (p -n <= x <= p)%Z.
+intros p n; functional induction ns p n.
+intros x [ | a l1].
+simpl; intros l2 np q; injection q;intros; omega.
+intros; destruct l1; discriminate.
+intros x [ | a l1];
+simpl; intros l2 np q; injection q; intros; try omega.
+assert (p - (n-1) <= x <= p)%Z.
+apply (IHl x l1 l2); auto; omega.
+omega.
+Qed.
+
+
+Lemma map_contiguous :
+forall A B : Type, forall f : A -> B, forall l,
+forall l1 l2 a b, map f l = l1++a::b::l2 ->
+  {l'1 :list A & {l'2 : list A & {x:A & {y:A | l1 = map f l'1 /\ l2= map f l'2 /\ a = f x /\
+        b = f y /\ l = l'1++x::y::l'2}}}}.
+intros A B f l; induction l.
+simpl; intros; destruct l1; discriminate.
+intros l1 l2 b1 b2; destruct l1 as [ | a' l1].
+  simpl; intros q.
+destruct l as [|a'' l]; try discriminate q; simpl in q.
+injection q; intros.
+exists nil; exists l; exists a; exists a''; auto.
+simpl; intros q.
+injection q; intros q' q''.
+destruct (IHl _ _ _ _ q') as [r1 [r2 [x [y [q1 [ q2 [qx [qy ql]]]]]]]].
+exists (a::r1); exists r2; exists x; exists y; repeat apply conj; auto.
+simpl; rewrite q'', q1; auto.
+simpl; rewrite ql; auto.
+Qed.
+
+Lemma map_app :
+  forall A B:Type, forall f : A -> B, forall l1 l2, map f (l1++l2) = map f l1 ++ map f l2.
+intros A B f l1; induction l1; simpl; auto.
+intros l2; rewrite IHl1; auto.
+Qed.
+
+Lemma non_empty_tail : 
+  forall (A:Type) (a:A) l, exists l', exists b, a::l = l'++(b::nil).
+intros A a l; generalize a; clear a; induction l.
+exists nil; exists a; auto.
+intros a'; destruct (IHl a) as [l' [b q]]; rewrite q.
+exists (a'::l'); exists b; auto.
+Qed.
+
+Lemma Qfrac_add_Z_l : forall a b c, (a#1) + (b#c) == (a*'c+b#c).
+intros;unfold Qeq; simpl; ring.
+Qed.
+
+Lemma constructive_mvt :
+  forall l x y, x < y -> eval_pol l x < 0 -> 0 <= eval_pol l y  ->
+       forall epsilon, 0 < epsilon ->
+       exists x', exists y',  -epsilon <= eval_pol l x' /\
+         eval_pol l x' < 0 /\ 0 <= eval_pol l y' /\
+         eval_pol l y' <= epsilon /\ x <= x' /\ x' < y' /\ y' <= y.
+intros l a b ab nla plb.
+destruct (translate_pol l a) as [l' q].
+assert (ba':0 < b-a).
+setoid_replace 0 with (a-a) by ring.
+unfold Qminus; repeat rewrite <- (Qplus_comm (-a));
+apply Qplus_le_lt_compat; auto.
+assert (ba:~ b-a == 0).
+intros abs; case (Qlt_not_eq 0 (b-a) ba'); rewrite abs; apply Qeq_refl.
+destruct (cm3 (b-a) ba' l') as [c pc].
+assert (mpolapos : 0 < -eval_pol l a) by (apply Qopp_lt_lr; assumption).
+assert (t1 : a-a == 0) by ring.
+assert (cpos: 0 < c).
+setoid_replace 0 with (0 */(b-a)) by ring.
+setoid_replace c with ((c*(b-a-(a-a)))/(b-a)) by (field;auto).
+apply Qmult_lt_compat_r; auto.
+apply Qlt_le_trans with (Qabs (eval_pol l' (b-a) - eval_pol l' (a-a))).
+match goal with |- 0 < Qabs(?a) => assert (ineq: 0 < a) end.
+repeat rewrite <- q; setoid_replace 0 with (0+0) by ring.
+apply Qplus_le_lt_compat; auto.
+rewrite pos_Qabs; auto.
+apply pc; try solve[rewrite t1; auto | auto].
+assert (cn0 : ~c==0) by (apply Qnot_eq_sym; apply Qlt_not_eq ; auto).
+intros epsilon pe.
+assert (en0 : ~ epsilon == 0) by (apply Qnot_eq_sym; apply Qlt_not_eq; auto).
+assert (pdiv: 0 < (b-a)*c/epsilon) by (repeat apply Qmult_lt_0_compat; auto).
+destruct (QZ_bound ((b-a)*c/(epsilon))) as [n qn]; auto.
+assert (pn : (0 < n)%Z).
+destruct ((b-a)*c/epsilon) as [nu de]; unfold Qle in qn, pdiv;
+simpl in qn, pdiv.  unfold Qlt in pdiv; simpl in pdiv; rewrite Zmult_1_r in pdiv, qn.
+assert (pdiv' := Zlt_le_trans _ _ _ pdiv qn).
+apply Zmult_lt_0_reg_r with ('de)%Z; try solve [compute; auto with zarith].
+assert (mkl: 
+  exists l, forall l1 l2 x y, a::l++b::nil = l1++x::y::l2 ->
+      y-x == (b-a)/(n#1) /\ exists k, x == a + (b-a)*(k#1)/(n#1) /\ (0<= k <= n-1)%Z).
+case (Z_eq_dec n 1).
+intros n1; exists nil; intros l1 l2 x y; destruct l1; simpl;
+  intros ql.
+injection ql; intros; subst x y n; split;
+ [field | exists 0%Z; split; [field | omega]].
+repeat (destruct l1; try discriminate).
+intros nn1; exists (map  (fun x => a + (b-a)*((x#1)/(n#1))) (ns (n-1) (n-2))).
+intros l1 l2  x y; destruct l1.
+assert (0 <= n-2)%Z by omega.
+destruct (ns_head (n-1) (n-2)) as [a1 qa1];auto; rewrite qa1; simpl.
+replace ((n-1)-(n-2))%Z with 1%Z by ring.
+intros ql; injection ql; intros; subst x y; split.
+field; unfold Qeq; simpl; omega.
+exists 0%Z; split;[field; unfold Qeq; simpl; omega | omega].
+simpl; intros q'; injection q'; clear q'.
+destruct l2 as [| d l2].
+replace (x::y::nil) with ((x::nil)++(y::nil)). rewrite  <- app_ass.
+intros q' _; elim (app_inj_tail  _ _ _ _ q'); clear q'; intros q' q''.
+destruct (ns_tail (n-1)(n-2)) as [l3 ql3].
+rewrite ql3 in q'.
+rewrite map_app in q'; simpl in q'.
+elim (app_inj_tail _ _ _ _ q'); clear q'; intros q' q3'.
+subst x y.
+assert (t0:(n-1#1)/(n#1) == 1 - /(n#1)).
+setoid_replace 1 with ((n#1)/(n#1)).
+setoid_replace (/(n#1)) with (1/(n#1)).
+unfold Qdiv.
+match goal with |- _ == ?a =>
+    setoid_replace a with (((n#1) - 1) * /(n#1)) by ring end.
+apply Qmult_comp.
+unfold Qeq; simpl; ring.
+apply Qeq_refl.
+field; unfold Qeq; simpl; omega.
+field; unfold Qeq; simpl; omega.
+rewrite t0.
+split.
+field; unfold Qeq; simpl; omega.
+exists (n-1)%Z; split.
+unfold Qdiv; rewrite Qmult_assoc; apply Qeq_refl.
+omega.
+simpl; auto.
+unfold Qdiv.
+destruct (non_empty_tail  _ d l2) as [l3 [e qe]].
+rewrite qe.
+replace (l1++x::y::l3++e::nil) with ((l1++x::y::l3)++(e::nil)).
+intros q' _.
+destruct (app_inj_tail _ _ _ _ q') as [q'' _].
+destruct (map_contiguous _ _ (fun x => a+(b-a)*((x#1)*/(n#1)))
+             _ _ _ _ _ q'') as [l'1 [l'2 [n1 [n2 [_ [_ [qx [qy st]]]]]]]].
+subst x y; setoid_replace (n2#1) with ((n1#1)+1).
+split.
+ring.
+exists n1; split. 
+rewrite Qmult_assoc; apply Qeq_refl.
+apply ns_bounds in st; omega.
+rewrite Qfrac_add_Z_l; rewrite Zmult_1_r.
+apply ns_step in st; try omega; rewrite st; apply Qeq_refl.
+rewrite app_ass; auto.
+destruct mkl as [sl qsl].
+destruct (find_pair Q (fun x => eval_pol l x < 0) 
+                  (fun x y => y - x == (b-a)/(n#1) /\
+                     exists k, x == a + (b-a)*(k#1) /(n#1) /\
+                     (0 <= k <= n-1)%Z)
+                 sl a b) 
+  as [a' [b' [[A1 [k [A4 A5]]][A2 A3]]]]; auto.
+apply Qle_not_lt; auto.
+intros x _; case (Qlt_le_dec (eval_pol l x) 0); auto.
+intros H; right; apply Qle_not_lt; auto.
+clear qsl sl.
+exists a'; exists b'.
+assert (aa':a <= a').
+(setoid_replace a with (a+0) by ring); rewrite A4.
+apply Qplus_le_compat; try apply Qle_refl.
+repeat apply Qmult_le_0_compat; auto.
+unfold Qle; simpl; omega.
+apply Qlt_le_weak; apply Qinv_lt_0_compat; unfold Qlt; simpl; omega.
+assert (bb': b' <= b).
+setoid_replace b with (a + (b-a) * (n#1) * /(n#1)) by
+ field; unfold Qeq; simpl; omega.
+(setoid_replace b' with (a' + (b' - a')) by ring); rewrite A1, A4.
+rewrite <- Qplus_assoc; apply Qplus_le_compat; try apply Qle_refl.
+unfold Qdiv;
+ match goal with |- ?f <= _ => setoid_replace f with ((b-a)* ((k#1)+1) * /(n#1))
+ end.
+apply Qmult_le_compat_r.
+repeat rewrite (Qmult_comm (b-a)); apply Qmult_le_compat_r.
+rewrite Qfrac_add_Z_l; unfold Qle; simpl; omega.
+auto.
+apply Qlt_le_weak; apply Qinv_lt_0_compat; unfold Qlt; simpl; omega.
+field; unfold Qeq; simpl; omega.
+assert (ab': a' < b').
+setoid_replace a' with (a' + 0) by ring.
+(setoid_replace b' with (a' + (b' - a')) by ring); rewrite A1.
+apply Qplus_le_lt_compat; try apply Qle_refl; apply Qmult_lt_0_compat; auto.
+apply Qinv_lt_0_compat; unfold Qlt; simpl; omega.
+assert (epsban: (b-a)*c / (n#1) <= epsilon).
+apply Qmult_lt_0_le_reg_r with ((n#1) / epsilon).
+apply Qmult_lt_0_compat; auto.
+unfold Qlt; simpl; omega.
+match goal with |- ?f1 <= ?f2 =>
+  (setoid_replace f2 with (n#1) by field; auto);
+  (setoid_replace f1 with ((b-a)*c /epsilon) by
+   (field; split; auto; unfold Qeq; simpl; omega)); auto
+end.
+split;[idtac | split; auto].
+(* start with epsilon and a'. *)
+apply Qopp_le_rl.
+apply Qle_trans with (eval_pol l b' - eval_pol l a').
+setoid_replace (-eval_pol l a') with (0 - eval_pol l a') by ring.
+apply Qplus_le_compat; auto; apply Qnot_lt_le; auto.
+repeat rewrite q.
+rewrite <- (pos_Qabs (eval_pol l' (b'-a) - eval_pol l' (a'-a))).
+apply Qle_trans with (c*((b'-a)-(a'-a))).
+apply pc; auto.
+(setoid_replace 0 with (a - a) by ring); apply Qplus_le_compat; auto; apply Qle_refl.
+apply Qplus_le_compat; auto.
+apply Qplus_le_compat; auto.
+setoid_replace (b' -a -(a'-a)) with (b' -a') by ring.
+rewrite A1.
+unfold Qdiv; rewrite Qmult_assoc; rewrite (Qmult_comm c); exact epsban.
+repeat rewrite <- q.
+(setoid_replace 0 with (0+0) by ring);apply Qplus_le_compat.
+apply Qnot_lt_le; auto.
+apply Qopp_le_lr.
+(setoid_replace 0 with (-0) by ring);apply Qlt_le_weak; assumption.
+split.
+apply Qnot_lt_le; auto.
+split; auto.
+apply Qle_trans with (eval_pol l' (b' -a) -eval_pol l' (a' -a)).
+setoid_replace (eval_pol l b') with (eval_pol l b' + 0) by ring.
+apply Qplus_le_compat.
+rewrite q; apply Qle_refl.
+rewrite <- q; apply Qopp_le_lr; auto.
+rewrite <- (pos_Qabs (eval_pol l' (b'-a) - eval_pol l' (a'-a))).
+apply Qle_trans with (c*((b'-a)-(a'-a))).
+apply pc; auto.
+(setoid_replace 0 with (a - a) by ring); apply Qplus_le_compat; auto; apply Qle_refl.
+apply Qplus_le_compat; auto.
+apply Qplus_le_compat; auto.
+setoid_replace (b' -a -(a'-a)) with (b' -a') by ring.
+rewrite A1.
+unfold Qdiv; rewrite Qmult_assoc; rewrite (Qmult_comm c); exact epsban.
+repeat rewrite <- q.
+(setoid_replace 0 with (0+0) by ring);apply Qplus_le_compat.
+apply Qnot_lt_le; auto.
+apply Qopp_le_lr.
+apply Qlt_le_weak; assumption.
+Qed.
